$$y' = f(x)g(y) $$
$$ M(x)N(y)dx+P(x)Q(y)dy=0 $$
$$x^2y^2y'+1=1 $$
$$ x^2y^2\dfrac{dx}{dy}=y-1$$
$$ \dfrac{y^2}{y-1}dy=\dfrac{dx}{x^2}$$
$$\sqrt{y^2+1}dx=xy dy$$
$$y'=\sqrt{4x+2y-1}$$
$$x\dfrac{dx}{dt}+t=1 $$
$$ \begin{cases}
    \dot{x}=y+2e^t \\
    \dot{y}=x+t^2
    \end{cases}
$$
$$\begin{cases}
    \dot{x}=2x+y+e^t \\
    \dot{y}=-2x+2t
\end{cases}
$$
$$
\dot x=Ax, \begin{pmatrix}
3&0\\
0&3
\end{pmatrix}
$$
$$
\dot x=Ax, \begin{pmatrix}
2&-1&-1\\
1&0&-1\\
3&-1&-2
\end{pmatrix}
$$
$$
\dot x=Ax, \begin{pmatrix}
3&-3&1\\
3&-2&2\\
-1&2&0
\end{pmatrix}
$$